src/FOL/ex/LocaleTest.thy
@@ -798,6 +798,9 @@ section {* Interpretation of Defined Concepts *}
 
 text {* Naming convention for global objects: prefixes D and d *}
 
+
+subsection {* Simple examples *}
+
 locale Da = fixes a :: o
   assumes true: a
 
@@ -807,7 +810,7 @@ lemma (in Da) not_false: "~ a <-> False"
   apply simp apply (rule true) done
 
 interpretation D1: Da ["True"]
-  where "~ True" = "False"
+  where "~ True == False"
   apply -
   apply unfold_locales [1] apply rule
   by simp
@@ -816,7 +819,7 @@ thm D1.not_false
 lemma "False <-> False" apply (rule D1.not_false) done
 
 interpretation D2: Da ["x | ~ x"]
-  where "~ (x | ~ x)" = "~ x & x"
+  where "~ (x | ~ x) <-> ~ x & x"
   apply -
   apply unfold_locales [1] apply fast
   by simp
